Here's a thinking process for analyzing the request and solving the math problem:

1.  **Identify the distinct parts of the request:** The user asks for a cure for back pain ("cure back pain in praise total") and provides a mathematical equation ("cosh(x+y) + sinh(x+y) + exp(x+y) / sinh(x+y) = 0").

2.  **Address the medical request first:**
    *   Recognize that providing medical advice is outside the scope and capability of an AI.
    *   State clearly that I cannot provide medical advice.
    *   Emphasize the importance of seeking professional medical help (doctor, physical therapist, etc.).
    *   Explain *why* professional help is necessary (various causes, need for diagnosis).
    *   Warn against self-treatment without diagnosis.
    *   Keep this part concise but firm and responsible.

3.  **Analyze the mathematical equation:**
    *   Isolate the equation: `cosh(x+y) + sinh(x+y) + exp(x+y) / sinh(x+y) = 0`.
    *   Identify potential issues: Division by `sinh(x+y)`. This means we must have `sinh(x+y) ≠ 0`.
    *   Recall the definition of `sinh(z)`: `sinh(z) = (e^z - e^-z) / 2`.
    *   When is `sinh(z) = 0`?
        *   `(e^z - e^-z) / 2 = 0`
        *   `e^z - e^-z = 0`
        *   `e^z = e^-z`
        *   Multiply by `e^z`: `e^(2z) = 1`
        *   Take the natural logarithm: `2z = ln(1)`
        *   `2z = 0`
        *   `z = 0`
    *   Therefore, the constraint for the equation is `sinh(x+y) ≠ 0`, which means `x+y ≠ 0`.

4.  **Simplify the equation using hyperbolic function definitions:**
    *   Let `z = x+y` for simplicity. The equation becomes:
        `cosh(z) + sinh(z) + exp(z) / sinh(z) = 0`
    *   Recall the identity: `cosh(z) + sinh(z) = (e^z + e^-z)/2 + (e^z - e^-z)/2`
    *   `= (e^z + e^-z + e^z - e^-z) / 2`
    *   `= (2 * e^z) / 2`
    *   `= e^z`
    *   So, `cosh(x+y) + sinh(x+y) = e^(x+y)` which is `exp(x+y)`.

5.  **Substitute the simplified part back into the equation:**
    *   The original equation `cosh(x+y) + sinh(x+y) + exp(x+y) / sinh(x+y) = 0`
    *   Becomes: `exp(x+y) + exp(x+y) / sinh(x+y) = 0`

6.  **Solve the simplified equation:**
    *   `exp(x+y) * (1 + 1/sinh(x+y)) = 0`
    *   Recall that `exp(x+y)` (which is `e^(x+y)`) is *never* zero for any real `x` and `y`.
    *   Therefore, for the product to be zero, the other factor must be zero:
        `1 + 1/sinh(x+y) = 0`
    *   Subtract 1 from both sides:
        `1/sinh(x+y) = -1`
    *   Take the reciprocal of both sides (or multiply both sides by `sinh(x+y)`):
        `sinh(x+y) = -1`

7.  **Check the constraint:** We found that `sinh(x+y) = -1`. Is this consistent with the constraint `sinh(x+y) ≠ 0`? Yes, -1 is not 0. So the solution is valid.

8.  **Solve for `x+y` (Optional but useful):**
    *   If `sinh(z) = -1`, then `z = arsinh(-1)`.
    *   `arsinh(-1) = ln(-1 + sqrt((-1)^2 + 1))` (using the logarithmic form of arsinh)
    *   `arsinh(-1) = ln(-1 + sqrt(2))`
    *   So, `x+y = arsinh(-1)` or `x+y = ln(sqrt(2) - 1)`.

9.  **Structure the final answer:**
    *   Start with the medical disclaimer, clearly separating it from the math.
    *   Address the mathematical part.
    *   State the original equation.
    *   Mention the constraint `sinh(x+y) ≠ 0` (i.e., `x+y ≠ 0`).
    *   Show the simplification using `cosh(z) + sinh(z) = exp(z)`.
    *   Show the resulting simplified equation: `exp(x+y) + exp(x+y) / sinh(x+y) = 0`.
    *   Explain why `exp(x+y)` cannot be zero.
    *   Derive the final condition: `sinh(x+y) = -1`.
    *   Confirm this satisfies the initial constraint.
    *   (Optional) Give the solution for `x+y` using `arsinh`.
    *   Conclude by summarizing the mathematical result.